factorial example whith recursion through the store, small fix to set_global rule, beginnings of a proofmode

theories/iris/examples/iris_example_helper.v
@@ -17,6 +17,26 @@ Close Scope byte_scope.
 (* Shorthands for common constructors *)
 Definition xx i := (VAL_int32 (Wasm_int.int_of_Z i32m i)).
 Definition xb b := (VAL_int32 (wasm_bool b)).
+Definition yy i := (Wasm_int.nat_of_uint i32m (Wasm_int.int_of_Z i32m i)).
+
+Section Examples.
+  Context `{!wasmG Σ}.
+  
+  (* Helper lemmas and tactics for necessary list manipulations for expressions *)
+  Lemma iRewrite_nil_l (s : stuckness) (E : coPset) (Φ : val -> iProp Σ) (e : iris.expr) :
+    (WP [] ++ e @ s; E {{ Φ }} ⊢ WP e @ s; E {{ Φ }}).
+  Proof. rewrite app_nil_l. auto. Qed.
+  Lemma iRewrite_nil_r (s : stuckness) (E : coPset) (Φ : val -> iProp Σ) (e : iris.expr) :
+    (WP e ++ [] @ s; E {{ Φ }} ⊢ WP e @ s; E {{ Φ }}).
+  Proof. rewrite app_nil_r. auto. Qed.
+  Lemma iRewrite_nil_l_ctx (s : stuckness) (E : coPset) (Φ : val -> iProp Σ) (e : iris.expr) i lh :
+    (WP [] ++ e @ s; E CTX i; lh {{ Φ }} ⊢ WP e @ s; E CTX i; lh {{ Φ }}).
+  Proof. rewrite app_nil_l. auto. Qed.
+  Lemma iRewrite_nil_r_ctx (s : stuckness) (E : coPset) (Φ : val -> iProp Σ) (e : iris.expr) i lh :
+    (WP e ++ [] @ s; E CTX i; lh {{ Φ }} ⊢ WP e @ s; E CTX i; lh {{ Φ }}).
+  Proof. rewrite app_nil_r. auto. Qed.
+
+End Examples.
 
 (* Tactics *)
 Ltac take_drop_app_rewrite n :=
@@ -30,7 +50,7 @@ Ltac take_drop_app_rewrite n :=
   | |- context [ WP ?e @ _; _ FRAME _; _ {{ _ }} %I ] =>
       rewrite -(list.take_drop n e);simpl take; simpl drop
   end.
-  
+
 Ltac take_drop_app_rewrite_twice n m :=
   take_drop_app_rewrite n;
   match goal with
