theories/iris/examples/iris_examples_factorial.v
@@ -1,0 +1,1048 @@
+From mathcomp Require Import ssreflect eqtype seq ssrbool.
+From iris.program_logic Require Import language.
+From iris.proofmode Require Import base tactics classes.
+From iris.base_logic Require Export gen_heap ghost_map proph_map.
+From iris.base_logic.lib Require Export fancy_updates.
+From iris.bi Require Export weakestpre.
+Require Export iris iris_locations iris_properties iris_atomicity stdpp_aux.
+Require Export iris_rules iris_example_helper iris_host proofmode.
+Require Export datatypes operations properties opsem.
+
+Set Implicit Arguments.
+Unset Strict Implicit.
+Unset Printing Implicit Defensive.
+
+Close Scope byte_scope.
+
+(* Example Programs *)
+Section Factorial.
+  Context `{!wasmG Σ}.
+
+  (* --------------------------------------------------------------------------------------------- *)
+  (* ------------------------- LOCAL STATE EXAMPLE: FACTORIAL ------------------------------------ *)
+  (* --------------------------------------------------------------------------------------------- *)
+
+  Definition factorial_instrs fact : seq.seq basic_instruction :=
+    [(BI_get_local 0);
+     (BI_const (xx 1));
+     (BI_relop T_i32 (Relop_i (ROI_le SX_U)));
+     (BI_if (Tf [] [T_i32])
+        [BI_const (xx 1)]
+        
+        [BI_get_local 0;
+         BI_const (xx 1);
+         BI_binop T_i32 (Binop_i BOI_sub);
+         BI_call fact;
+         BI_get_local 0;
+         BI_binop T_i32 (Binop_i BOI_mul)])].
+  Definition factorial fact := to_e_list (factorial_instrs fact).
+
+  Lemma factPred:
+    ∀ n : nat, 1 < n -> ssrnat.muln n (ssrnat.factorial (n - 1)) = (ssrnat.factorial n).
+  Proof.
+    intros n Hlt.
+    induction n. lia.
+    destruct n;[lia|].
+    destruct n;auto.
+  Qed.
+
+  Definition fact_val n : val -> iProp Σ := λ v, ⌜v = immV [xx (ssrnat.factorial (Wasm_int.nat_of_uint i32m n))]⌝%I.
+
+  Lemma factorial_spec fact (n : Equality.sort i32) i a :
+    (ssrnat.factorial (Wasm_int.nat_of_uint i32m n) < Wasm_int.Int32.modulus)%Z -> (* no overflow *)
+    inst_funcs i !! fact = Some a -> (* factorial function is in the instance *)
+    (0 <= (Wasm_int.Int32.intval n))%Z -> (* the parameter must be positive *)
+    
+    ↪[frame] Build_frame [VAL_int32 n] i -∗
+    (N.of_nat a) ↦[wf] (FC_func_native i (Tf [T_i32] [T_i32]) [] (factorial_instrs fact)) -∗
+    WP factorial fact {{ v, (fact_val n v
+                             ∗ (N.of_nat a) ↦[wf] (FC_func_native i (Tf [T_i32] [T_i32]) [] (factorial_instrs fact)))
+                             ∗ ↪[frame] Build_frame [VAL_int32 n] i }}.
+  Proof.
+    iLöb as "IH" forall (n).
+  { (* { is to fix annoying indent problem... *)
+    iIntros (Hoverflow Hle Ha) "Hf Hi".
+    rewrite /factorial.
+    iSimpl.
+    set f := {| f_locs := [VAL_int32 n]; f_inst := i |}.
+    match goal with
+    | |- context [ (▷ ?H)%I ] => set IH := H
+    end.
+
+    (* get_local 0 *)
+    take_drop_app_rewrite 1.
+    iApply (wp_seq _ _ _ (λ v', ⌜v' = immV _⌝ ∗ ↪[frame] f)%I).
+    iSplitR;[by iIntros "[%Hcontr _]"|].
+    iSplitL "Hf".
+    { iApply (wp_get_local with "[] [$]"). unfold f. eauto.
+      simpl. eauto. }
+    
+    (* le *)
+    iIntros (w) "[-> Hf] /=".
+    take_drop_app_rewrite 3.
+    iApply (wp_seq _ _ _ (λ v', ⌜v' = immV [_]⌝ ∗ ↪[frame] f)%I).
+    iSplitR;[by iIntros "[%Hcontr _]"|].
+    iSplitL "Hf".
+    { iApply (wp_relop with "[$]"). eauto. eauto. }
+
+    (* br if *)
+    iIntros (w) "[-> Hf] /=".
+    (* case distinction *)
+    destruct (~~ Wasm_int.Int32.ltu (Wasm_int.Int32.repr 1) n) eqn:Hbool;simpl.
+    { (* base case: n <= 1 *)
+      (* setup the true branch *)
+      apply negb_true in Hbool.
+      iApply (wp_if_true with "[$]");[auto|]. simpl.
+      iNext. iIntros "Hf".
+      iApply iRewrite_nil_l.
+      iApply (wp_block with "[$]");eauto.
+      iNext. iIntros "Hf".
+      iApply wp_wasm_empty_ctx.
+      iApply wp_label_push_nil. simpl.
+
+      (* return from block *)
+      iApply (wp_val_return with "[$]");auto.
+
+      (* halt and post condition *)
+      iIntros "Hf".
+      simpl. iApply (iris_wp.wp_value _ _ _ _ (immV ([xx 1]))). by cbv.
+      iFrame. iPureIntro. f_equiv. f_equiv.
+      unfold xx. f_equiv. f_equiv. clear -Hle Hbool.
+      destruct n;simpl in *.
+      unfold Wasm_int.Int32.ltu in Hbool. simpl in *.
+      destruct (Coqlib.zlt 1 intval);[done|].
+      assert (intval = 1 ∨ intval = 0);[lia|].
+      destruct H as [-> | ->];lias. }
+
+    { (* inductive step *)
+      (* setup the false branch *)
+      apply negbFE in Hbool.
+      iApply (wp_if_false with "[$]");[auto|].
+      iNext. iIntros "Hf".
+      iApply iRewrite_nil_l.
+      iApply (wp_block with "[$]");eauto.
+      iNext. iIntros "Hf".
+      iApply wp_wasm_empty_ctx.
+      iApply wp_label_push_nil. simpl.
+
+      (* get_local 0 *)
+      take_drop_app_rewrite 1.
+      iApply (wp_seq_ctx _ _ _ (λ v', ⌜v' = immV _⌝ ∗ ↪[frame] f)%I).
+      iSplitR; [by iIntros "[%Hcontr _]"|].
+      iSplitL "Hf".
+      { iApply (wp_get_local with "[] [$]"). unfold f. eauto.
+        simpl. eauto. }
+
+      (* sub *)
+      iIntros (w) "[-> Hf] /=".
+      take_drop_app_rewrite 3.
+      iApply (wp_seq_ctx _ _ _ (λ v', ⌜v' = immV _⌝ ∗ ↪[frame] f)%I).
+      iSplitR; [by iIntros "[%Hcontr _]"|].
+      iSplitL "Hf".
+      { iApply (wp_binop with "[$]"). eauto. eauto. }
+
+      (* recursive call *)
+      simpl.
+      iIntros (w) "[-> Hf] /=".
+      take_drop_app_rewrite 2.
+      iApply (wp_seq_ctx _ _ _ (λ v', (⌜v' = immV _⌝ ∗ N.of_nat a ↦[wf] _) ∗ ↪[frame] f)%I).
+      iSplitR; [by iIntros "[[%Hcontr _] _]"|].
+      iSplitL.
+      { (* call *)
+        iApply wp_wasm_empty_ctx.
+        take_drop_app_rewrite_twice 1 0.
+        iApply wp_base_push;auto. simpl.
+        iApply (wp_call_ctx with "[$]"). unfold f. simpl. eauto.
+        iNext. iIntros "Hf".
+
+        (* invoke native *)
+        iApply wp_base. simpl.
+        take_drop_app_rewrite 1.
+        iApply (wp_invoke_native with "Hf Hi");eauto.
+        iNext. iIntros "[Hf Hi]".
+        simpl.
+
+        (* scope change before invoking the IH *)
+        rewrite -wp_frame_rewrite.
+        iApply wp_wasm_empty_ctx_frame.
+        take_drop_app_rewrite 1.
+        iApply (wp_seq_ctx_frame _ _ _ (λ v', ⌜v' = immV _⌝ ∗ N.of_nat a ↦[wf] _)%I with "[$Hf Hi]").
+        { intros LI HLI%lfilled_Ind_Equivalent. inversion HLI;subst. cbn. auto. }
+        iSplitR; [by iIntros "[%Hcontr _]"|].
+        iSplitL.
+        { (* focus on block *)
+          iIntros "Hf".
+          take_drop_app_rewrite 0.
+          iApply (wp_block with "[$]");eauto.
+          iNext. iIntros "Hf".
+          iApply wp_wasm_empty_ctx.
+          assert ([] ++ to_e_list (factorial_instrs fact) =
+                    ([] ++ to_e_list (factorial_instrs fact) ++ []))%SEQ as ->;[auto|].
+          iApply wp_label_push;auto.
+          iApply iRewrite_nil_r_ctx.
+          iApply wp_seq_ctx.
+          iSplitR;cycle 1.
+          { iSplitL. (* apply IH *)
+            unfold IH.
+            iApply ("IH" with "[] [] [] Hf Hi");auto.
+            - iPureIntro.
+              (* prove that (n - 1) does not overflow *)
+              clear -Ha Hbool Hoverflow.
+              destruct n. simpl in *.
+              unfold Wasm_int.Int32.ltu in Hbool. simpl in *.
+              destruct (Coqlib.zlt 1 intval);[|done].
+              rewrite Wasm_int.Int32.Z_mod_modulus_eq Zmod_small;try lia.
+              rewrite Z2Nat.inj_sub;[|lia].
+              rewrite (Nat2Z.id 1).
+              apply Zmult_gt_0_lt_reg_r with (p:=intval). lia.
+              assert ((ssrnat.factorial (Z.to_nat intval - 1) * intval)%Z
+                      = ssrnat.muln (Z.to_nat intval) (ssrnat.factorial (Z.to_nat intval - 1))) as Heq.
+              { unfold ssrnat.muln. unfold ssrnat.muln_rec. lia. }
+              rewrite Heq factPred;[|lia]. etrans. apply Hoverflow.
+              apply Z.lt_mul_diag_r;lia.
+              
+            - iPureIntro.
+              (* prove that (n - 1) is gt 0 *)
+              clear -Ha Hbool.
+              destruct n. simpl in *.
+              unfold Wasm_int.Int32.ltu in Hbool. simpl in *.
+              destruct (Coqlib.zlt 1 intval);[|done].
+              rewrite Wasm_int.Int32.Z_mod_modulus_eq Zmod_small;lia.
+
+            - (* return *)
+              iIntros (w) "[[-> Hi] Hf] /=".
+              iApply (wp_val_return with "[$] [Hi]"). auto.
+              iIntros "Hf /=".
+              iApply iris_wp.wp_value. instantiate (1 := immV [_]). reflexivity.
+              iFrame. eauto. }
+          { simpl. by iIntros "[[%Hcontr _] _]". } }
+
+        (* return to outer scope *)
+        iIntros (w) "[[-> Hi] Hf] /=".
+        iApply wp_wasm_empty_ctx_frame.
+        rewrite wp_frame_rewrite.
+        iApply (wp_frame_value with "[$Hf]"); eauto.
+      }
+      
+      (* finish program after call *)
+      iIntros (w) "[[-> Hi] Hf] /=".
+      
+      (* get_local 0 *)
+      take_drop_app_rewrite_twice 1 1.
+      iApply wp_base_push;auto.
+      take_drop_app_rewrite 1.
+      iApply (wp_seq_ctx _ _ _ (λ v', ⌜v' = immV _⌝ ∗ ↪[frame]f)%I).
+      iSplitR;[by iIntros "[%Hcontr _]"|].
+      iSplitL "Hf".
+      { iApply (wp_get_local with "[] [$Hf]"). eauto. simpl. eauto. }
+
+      (* mul *)
+      iIntros (w) "[-> Hf] /=".
+      iApply wp_base_pull. simpl.
+      take_drop_app_rewrite 3.
+      iApply (wp_seq_ctx _ _ _ (λ v', ⌜v' = immV _⌝ ∗ ↪[frame] f)%I).
+      iSplitR;[by iIntros "[%Hcontr _]"|].
+      iSplitL "Hf".
+      { iApply (wp_binop with "[$]"). simpl. eauto. eauto. }
+
+      (* return *)
+      iIntros (w) "[-> Hf] /=".
+      iApply (wp_val_return with "[$]");auto.
+      iIntros "Hf /=".
+
+      (* postcondition *)
+      iApply iris_wp.wp_value. instantiate (1 := immV [_]). reflexivity.
+      iFrame. iPureIntro.
+
+      unfold xx.
+      repeat f_equiv.
+      unfold Wasm_int.Int32.imul, Wasm_int.Int32.mul. simpl.
+      f_equiv.
+      clear -Ha Hbool Hoverflow.
+      unfold Wasm_int.Int32.ltu in Hbool.
+      destruct n;simpl in *.
+      destruct (Coqlib.zlt 1 intval);[|done].
+      rewrite !Wasm_int.Int32.Z_mod_modulus_eq.
+      assert ((intval - 1) `mod` Wasm_int.Int32.modulus = intval - 1)%Z as ->.
+      { rewrite Zmod_small;lia. }
+      rewrite Z2Nat.inj_sub;[|lia].
+      rewrite (Nat2Z.id 1).
+      assert ((ssrnat.factorial (Z.to_nat intval - 1) * intval)%Z
+              = ssrnat.muln (Z.to_nat intval) (ssrnat.factorial (Z.to_nat intval - 1))) as Heq.
+      { unfold ssrnat.muln. unfold ssrnat.muln_rec. lia. }
+      rewrite Zmod_small.
+      rewrite Heq factPred;lia.
+      split. lia.
+      apply Zmult_gt_0_lt_reg_r with (p:=intval). lia.
+      rewrite Heq factPred. 2: lia.
+      etrans. apply Hoverflow.
+      apply Z.lt_mul_diag_r;lia.
+  } }
+  Qed.
+
+  Lemma invoke_factorial_spec fact (n : Equality.sort i32) i a f0 :
+    (ssrnat.factorial (Wasm_int.nat_of_uint i32m n) < Wasm_int.Int32.modulus)%Z -> (* no overflow *)
+    inst_funcs i !! fact = Some a -> (* factorial function is in the instance *)
+    (0 <= (Wasm_int.Int32.intval n))%Z -> (* the parameter must be positive *)
+    
+    ↪[frame] f0 -∗
+    (N.of_nat a) ↦[wf] (FC_func_native i (Tf [T_i32] [T_i32]) [] (factorial_instrs fact)) -∗
+    WP [AI_basic (BI_const (VAL_int32 n));
+        AI_invoke a]
+    {{ v, (⌜v = immV [xx (ssrnat.factorial (Wasm_int.nat_of_uint i32m n))]⌝
+            ∗ (N.of_nat a) ↦[wf] (FC_func_native i (Tf [T_i32] [T_i32]) [] (factorial_instrs fact)))
+            ∗ ↪[frame] f0 }}.
+  Proof.
+    iIntros (Hoverflow Hi Hpos) "Hf Hi".
+    take_drop_app_rewrite 1.
+    iApply (wp_invoke_native with "[$] [$]");eauto.
+    iNext. iIntros "[Hf Hi]".
+    rewrite /= -wp_frame_rewrite.
+    iApply wp_wasm_empty_ctx_frame.
+    take_drop_app_rewrite 1.
+    iApply (wp_seq_ctx_frame _ _ _ (λ v, fact_val n v ∗ (N.of_nat a) ↦[wf] _)%I with "[$Hf Hi]").
+    { intros LI HLI%lfilled_Ind_Equivalent. inversion HLI;subst. cbn. auto. }
+    iSplitR;[by iIntros "[%Hcontr _]"|].
+    iSplitL.
+    { iIntros "Hf".
+      take_drop_app_rewrite 0.
+      iApply (wp_block with "[$]");eauto.
+      iNext. iIntros "Hf".
+      erewrite app_nil_l.
+      iApply wp_wasm_empty_ctx.
+      iApply wp_label_push_nil. simpl push_base.
+      take_drop_app_rewrite (length (factorial_instrs fact)).
+      iApply (wp_seq_ctx _ _ _ (λ v, (fact_val n v ∗ (N.of_nat a) ↦[wf] _) ∗ ↪[frame] _)%I).
+      iSplitR;[by iIntros "[[%Hcontr _] _]"|].
+      iSplitL.
+      { iApply (factorial_spec with "[$] [$]");eauto. }
+      iIntros (w) "[[%Hfact Hi] Hf] /=".
+      iApply (wp_val_return with "[$]");[subst;auto|].
+      iIntros "Hf /=".
+      iApply iris_wp.wp_value. instantiate (1:=immV [_]). subst;done.
+      iFrame. auto. }
+    iIntros (w) "[[%Hfact Hi] Hf]".
+    iApply wp_wasm_empty_ctx_frame.
+    iApply (wp_frame_value with "[$]"); [subst;eauto..|].
+    iNext.
+    iFrame. auto.
+  Qed.
+
+End Factorial.
+
+Section Factorial.
+  Context `{!wasmG Σ}.
+  
+  (* --------------------------------------------------------------------------------------------- *)
+  (* ------------------------- LANDIN'S KNOT EXAMPLE: FACTORIAL ---------------------------------- *)
+  (* --------------------------------------------------------------------------------------------- *)
+
+
+  Definition myrec_instr h_mut_tab :=
+    [BI_const (xx 0);
+     BI_get_local 0;
+     BI_call h_mut_tab].
+  Definition myrec h_mut_tab := to_e_list (myrec_instr h_mut_tab).
+
+  Definition F_instr rec_typ :=
+    [(BI_get_local 0);
+     (BI_const (xx 1));
+     (BI_relop T_i32 (Relop_i (ROI_le SX_U)));
+     (BI_if (Tf [] [T_i32])
+        [BI_const (xx 1)]
+        
+        [BI_get_local 0;
+         BI_const (xx 1);
+         BI_binop T_i32 (Binop_i BOI_sub);
+         BI_const (xx 0);
+         BI_call_indirect rec_typ;
+         BI_get_local 0;
+         BI_binop T_i32 (Binop_i BOI_mul)])].
+  Definition F rec_typ :=
+    to_e_list (F_instr rec_typ).
+
+  Definition fact_instr F myrec fact_typ :=
+    [BI_get_local 0;
+     BI_const F;
+     BI_call myrec;
+     BI_const (xx 0);
+     BI_call_indirect fact_typ].
+  Definition fact F myrec fact_typ :=
+    to_e_list (fact_instr F myrec fact_typ).
+
+  
+  Lemma F_spec fact rec_typ tab (n : Equality.sort i32) i a :
+    (ssrnat.factorial (Wasm_int.nat_of_uint i32m n) < Wasm_int.Int32.modulus)%Z -> (* no overflow *)
+    (0 <= (Wasm_int.Int32.intval n))%Z -> (* the parameter must be positive *)
+
+    inst_funcs i !! fact = Some a -> (* factorial function is in the instance *)
+    inst_types i !! rec_typ = Some (Tf [T_i32] [T_i32]) ->
+    inst_tab i !!  0 = Some tab ->
+    
+    ↪[frame] Build_frame [VAL_int32 n] i -∗
+    (N.of_nat tab) ↦[wt][N.of_nat (yy 0)] Some a -∗
+    (N.of_nat a) ↦[wf] (FC_func_native i (Tf [T_i32] [T_i32]) [] (F_instr rec_typ)) -∗
+    WP F rec_typ {{ v, (fact_val n v
+                             ∗ (N.of_nat tab) ↦[wt][N.of_nat (yy 0)] Some a 
+                             ∗ (N.of_nat a) ↦[wf] (FC_func_native i (Tf [T_i32] [T_i32]) [] (F_instr rec_typ)))
+                             ∗ ↪[frame] Build_frame [VAL_int32 n] i }}.
+  Proof.
+    iLöb as "IH" forall (n).
+  { (* { is to fix annoying indent problem... *)
+    iIntros (Hoverflow Hle Ha Htyp Htab) "Hf Htab Hi".
+    rewrite /F.
+    iSimpl.
+    set f := {| f_locs := [VAL_int32 n]; f_inst := i |}.
+    match goal with
+    | |- context [ (▷ ?H)%I ] => set IH := H
+    end.
+
+    (* get_local 0 *)
+    take_drop_app_rewrite 1.
+    iApply (wp_seq _ _ _ (λ v', ⌜v' = immV _⌝ ∗ ↪[frame] f)%I).
+    iSplitR;[by iIntros "[%Hcontr _]"|].
+    iSplitL "Hf".
+    { iApply (wp_get_local with "[] [$]"). unfold f. eauto.
+      simpl. eauto. }
+    
+    (* le *)
+    iIntros (w) "[-> Hf] /=".
+    take_drop_app_rewrite 3.
+    iApply (wp_seq _ _ _ (λ v', ⌜v' = immV [_]⌝ ∗ ↪[frame] f)%I).
+    iSplitR;[by iIntros "[%Hcontr _]"|].
+    iSplitL "Hf".
+    { iApply (wp_relop with "[$]"). eauto. eauto. }
+
+    (* br if *)
+    iIntros (w) "[-> Hf] /=".
+    (* case distinction *)
+    destruct (~~ Wasm_int.Int32.ltu (Wasm_int.Int32.repr 1) n) eqn:Hbool;simpl.
+    { (* base case: n <= 1 *)
+      (* setup the true branch *)
+      apply negb_true in Hbool.
+      iApply (wp_if_true with "[$]");[auto|]. simpl.
+      iNext. iIntros "Hf".
+      iApply iRewrite_nil_l.
+      iApply (wp_block with "[$]");eauto.
+      iNext. iIntros "Hf".
+      iApply wp_wasm_empty_ctx.
+      iApply wp_label_push_nil. simpl.
+
+      (* return from block *)
+      iApply (wp_val_return with "[$]");auto.
+
+      (* halt and post condition *)
+      iIntros "Hf".
+      simpl. iApply (iris_wp.wp_value _ _ _ _ (immV ([xx 1]))). by cbv.
+      iFrame. iPureIntro. f_equiv. f_equiv.
+      unfold xx. f_equiv. f_equiv. clear -Hle Hbool.
+      destruct n;simpl in *.
+      unfold Wasm_int.Int32.ltu in Hbool. simpl in *.
+      destruct (Coqlib.zlt 1 intval);[done|].
+      assert (intval = 1 ∨ intval = 0);[lia|].
+      destruct H as [-> | ->];lias. }
+
+    { (* inductive step *)
+      (* setup the false branch *)
+      apply negbFE in Hbool.
+      iApply (wp_if_false with "[$]");[auto|].
+      iNext. iIntros "Hf".
+      iApply iRewrite_nil_l.
+      iApply (wp_block with "[$]");eauto.
+      iNext. iIntros "Hf".
+      iApply wp_wasm_empty_ctx.
+      iApply wp_label_push_nil. simpl.
+
+      (* get_local 0 *)
+      take_drop_app_rewrite 1.
+      iApply (wp_seq_ctx _ _ _ (λ v', ⌜v' = immV _⌝ ∗ ↪[frame] f)%I).
+      iSplitR; [by iIntros "[%Hcontr _]"|].
+      iSplitL "Hf".
+      { iApply (wp_get_local with "[] [$]"). unfold f. eauto.
+        simpl. eauto. }
+
+      (* sub *)
+      iIntros (w) "[-> Hf] /=".
+      take_drop_app_rewrite 3.
+      iApply (wp_seq_ctx _ _ _ (λ v', ⌜v' = immV _⌝ ∗ ↪[frame] f)%I).
+      iSplitR; [by iIntros "[%Hcontr _]"|].
+      iSplitL "Hf".
+      { iApply (wp_binop with "[$]"). eauto. eauto. }
+
+      (* recursive call: now happens indirectly through the higher order store *)
+      simpl.
+      iIntros (w) "[-> Hf] /=".
+      take_drop_app_rewrite 3.
+      iApply (wp_seq_ctx _ _ _ (λ v', (⌜v' = immV _⌝ ∗ N.of_nat tab↦[wt][0%N]Some a ∗ N.of_nat a ↦[wf] _) ∗ ↪[frame] f)%I).
+      iSplitR; [by iIntros "[[%Hcontr _] _]"|].
+      iSplitL.
+      { (* call *)
+        iApply wp_wasm_empty_ctx.
+        take_drop_app_rewrite_twice 1 0.
+        iApply wp_base_push;auto. simpl.
+        iApply (wp_call_indirect_success_ctx with "[Htab] [$] [$]");auto. unfold f. simpl. eauto.
+        iNext. iIntros "[Htab [Hi Hf]]".
+
+        (* invoke native *)
+        iApply wp_base. simpl.
+        take_drop_app_rewrite 1.
+        iApply (wp_invoke_native with "Hf Hi");eauto.
+        iNext. iIntros "[Hf Hi]".
+        simpl.
+
+        (* scope change before invoking the IH *)
+        rewrite -wp_frame_rewrite.
+        iApply wp_wasm_empty_ctx_frame.
+        take_drop_app_rewrite 1.
+        iApply (wp_seq_ctx_frame _ _ _ (λ v', ⌜v' = immV _⌝ ∗ N.of_nat tab ↦[wt][0%N]Some a ∗ N.of_nat a ↦[wf] _)%I with "[$Hf Hi Htab]").
+        { intros LI HLI%lfilled_Ind_Equivalent. inversion HLI;subst. cbn. auto. }
+        iSplitR; [by iIntros "[%Hcontr _]"|].
+        iSplitL.
+        { (* focus on block *)
+          iIntros "Hf".
+          take_drop_app_rewrite 0.
+          iApply (wp_block with "[$]");eauto.
+          iNext. iIntros "Hf".
+          iApply wp_wasm_empty_ctx.
+          assert ([] ++ to_e_list (F_instr rec_typ) =
+                    ([] ++ to_e_list (F_instr rec_typ) ++ []))%SEQ as ->;[auto|].
+          iApply wp_label_push;auto.
+          iApply iRewrite_nil_r_ctx.
+          iApply wp_seq_ctx.
+          iSplitR;cycle 1.
+          { iSplitL. (* apply IH *)
+            unfold IH.
+            iApply ("IH" with "[] [] [] [] [] Hf Htab Hi");auto.
+            - iPureIntro.
+              (* prove that (n - 1) does not overflow *)
+              clear -Ha Hbool Hoverflow.
+              destruct n. simpl in *.
+              unfold Wasm_int.Int32.ltu in Hbool. simpl in *.
+              destruct (Coqlib.zlt 1 intval);[|done].
+              rewrite Wasm_int.Int32.Z_mod_modulus_eq Zmod_small;try lia.
+              rewrite Z2Nat.inj_sub;[|lia].
+              rewrite (Nat2Z.id 1).
+              apply Zmult_gt_0_lt_reg_r with (p:=intval). lia.
+              assert ((ssrnat.factorial (Z.to_nat intval - 1) * intval)%Z
+                      = ssrnat.muln (Z.to_nat intval) (ssrnat.factorial (Z.to_nat intval - 1))) as Heq.
+              { unfold ssrnat.muln. unfold ssrnat.muln_rec. lia. }
+              rewrite Heq factPred;[|lia]. etrans. apply Hoverflow.
+              apply Z.lt_mul_diag_r;lia.
+              
+            - iPureIntro.
+              (* prove that (n - 1) is gt 0 *)
+              clear -Ha Hbool.
+              destruct n. simpl in *.
+              unfold Wasm_int.Int32.ltu in Hbool. simpl in *.
+              destruct (Coqlib.zlt 1 intval);[|done].
+              rewrite Wasm_int.Int32.Z_mod_modulus_eq Zmod_small;lia.
+
+            - (* return *)
+              iIntros (w) "[[-> [Htab Hi]] Hf] /=".
+              iApply (wp_val_return with "[$] [Hi Htab]"). auto.
+              iIntros "Hf /=".
+              iApply iris_wp.wp_value. instantiate (1 := immV [_]). reflexivity.
+              iFrame. eauto. }
+          { simpl. by iIntros "[[%Hcontr _] _]". } }
+
+        (* return to outer scope *)
+        iIntros (w) "[[-> [Htab Hi]] Hf] /=".
+        iApply wp_wasm_empty_ctx_frame.
+        rewrite wp_frame_rewrite.
+        iApply (wp_frame_value with "[$Hf]"); eauto. iFrame. eauto.
+      }
+      
+      (* finish program after call *)
+      iIntros (w) "[[-> Hi] Hf] /=".
+      
+      (* get_local 0 *)
+      take_drop_app_rewrite_twice 1 1.
+      iApply wp_base_push;auto.
+      take_drop_app_rewrite 1.
+      iApply (wp_seq_ctx _ _ _ (λ v', ⌜v' = immV _⌝ ∗ ↪[frame]f)%I).
+      iSplitR;[by iIntros "[%Hcontr _]"|].
+      iSplitL "Hf".
+      { iApply (wp_get_local with "[] [$Hf]"). eauto. simpl. eauto. }
+
+      (* mul *)
+      iIntros (w) "[-> Hf] /=".
+      iApply wp_base_pull. simpl.
+      take_drop_app_rewrite 3.
+      iApply (wp_seq_ctx _ _ _ (λ v', ⌜v' = immV _⌝ ∗ ↪[frame] f)%I).
+      iSplitR;[by iIntros "[%Hcontr _]"|].
+      iSplitL "Hf".
+      { iApply (wp_binop with "[$]"). simpl. eauto. eauto. }
+
+      (* return *)
+      iIntros (w) "[-> Hf] /=".
+      iApply (wp_val_return with "[$]");auto.
+      iIntros "Hf /=".
+
+      (* postcondition *)
+      iApply iris_wp.wp_value. instantiate (1 := immV [_]). reflexivity.
+      iFrame. iPureIntro.
+
+      unfold xx.
+      repeat f_equiv.
+      unfold Wasm_int.Int32.imul, Wasm_int.Int32.mul. simpl.
+      f_equiv.
+      clear -Ha Hbool Hoverflow.
+      unfold Wasm_int.Int32.ltu in Hbool.
+      destruct n;simpl in *.
+      destruct (Coqlib.zlt 1 intval);[|done].
+      rewrite !Wasm_int.Int32.Z_mod_modulus_eq.
+      assert ((intval - 1) `mod` Wasm_int.Int32.modulus = intval - 1)%Z as ->.
+      { rewrite Zmod_small;lia. }
+      rewrite Z2Nat.inj_sub;[|lia].
+      rewrite (Nat2Z.id 1).
+      assert ((ssrnat.factorial (Z.to_nat intval - 1) * intval)%Z
+              = ssrnat.muln (Z.to_nat intval) (ssrnat.factorial (Z.to_nat intval - 1))) as Heq.
+      { unfold ssrnat.muln. unfold ssrnat.muln_rec. lia. }
+      rewrite Zmod_small.
+      rewrite Heq factPred;lia.
+      split. lia.
+      apply Zmult_gt_0_lt_reg_r with (p:=intval). lia.
+      rewrite Heq factPred. 2: lia.
+      etrans. apply Hoverflow.
+      apply Z.lt_mul_diag_r;lia.
+  } }
+  Qed.
+
+  Lemma myrec_spec h_mut_tab a mut_tab fidx i :
+    inst_funcs i !! h_mut_tab = Some a -> (* modify table host call is in the instance *)
+
+    ↪[frame] Build_frame [fidx] i -∗
+    N.of_nat a↦[wf]FC_func_host (Tf [T_i32; T_i32] []) mut_tab -∗
+    WP myrec h_mut_tab {{ v, (⌜v = callHostV (Tf [T_i32; T_i32] []) mut_tab [xx 0; fidx] (LL_base [] [])⌝
+                             ∗ N.of_nat a↦[wf]FC_func_host (Tf [T_i32; T_i32] []) mut_tab) ∗ ↪[frame] Build_frame [fidx] i }}.
+  Proof.
+    iIntros (Hh) "Hf Ha".
+    take_drop_app_rewrite_twice 1 1.
+
+    iApply wp_wasm_empty_ctx.
+    iApply wp_base_push;auto. simpl.
+    take_drop_app_rewrite 1.
+
+    (* get_local 0 *)
+    iApply (wp_seq_ctx _ _ _ (λ v, ⌜v = immV _⌝ ∗ _)%I).
+    iSplitR;[by iIntros "[%Hcontr _]"|].
+    iSplitL "Hf".
+    { iApply (wp_get_local with "[] [$]");eauto. }
+    iIntros (w) "[-> Hf] /=".
+
+    iApply wp_base_pull.
+    take_drop_app_rewrite_twice 2 0.
+    iApply wp_base_push;auto.
+
+    iApply (wp_call_ctx with "[$]");eauto.
+    iNext. iIntros "Hf".
+
+    iApply wp_base_pull.
+    iApply wp_wasm_empty_ctx. simpl.
+    take_drop_app_rewrite 2.
+    iApply (wp_invoke_host _ _ _ [xx 0; fidx] with "[$] [$]");auto. 
+    iNext. iIntros "Ha Hf".
+    iApply iris_wp.wp_value;[apply iris.of_to_val; eauto|].
+    iFrame. auto.
+  Qed.
+
+End Factorial.
+
+Section FactorialHostMain.
+  Context `{!wasmG Σ, !hvisG Σ, !hmsG Σ, !hasG Σ}.
+
+  Definition main_instr fact glob :=
+    [BI_get_global glob;
+     BI_call fact;
+     BI_set_global glob].
+  Definition main fact glob := to_e_list (main_instr fact glob).
+
+  Lemma main_host_spec fact glob F myrec tab mut_tab f_fact f_F f_myrec f_mut_tab g_glob t_fact_typ mt i tabval n idnstart f Φ :
+    inst_funcs i !! fact = Some f_fact ->
+    inst_funcs i !! (Wasm_int.nat_of_uint i32m F) = Some f_F ->
+    inst_funcs i !! myrec = Some f_myrec ->
+    inst_funcs i !! mut_tab = Some f_mut_tab ->
+    inst_types i !! t_fact_typ = Some (Tf [T_i32] [T_i32]) ->
+    inst_tab i !! 0 = Some tab ->
+    inst_globs i !! glob = Some g_glob ->
+
+    (ssrnat.factorial (Wasm_int.nat_of_uint i32m n) < Wasm_int.Int32.modulus)%Z -> (* no overflow *)
+    (0 <= (Wasm_int.Int32.intval n))%Z -> (* the parameter must be positive *)
+
+    (∀ v : host_val, ⌜v = immHV []⌝ ∗ (∃ w : value, fact_val n (immV [w]) ∗ (N.of_nat g_glob) ↦[wg] {| g_mut := MUT_mut; g_val := w |}) -∗ Φ v) -∗
+    ↪[frame] (* Build_frame [] i *) f -∗
+    (N.of_nat f_fact) ↦[wf] FC_func_native i (Tf [T_i32] [T_i32]) [] (fact_instr (VAL_int32 F) myrec t_fact_typ) -∗
+    (N.of_nat f_F) ↦[wf] FC_func_native i (Tf [T_i32] [T_i32]) [] (F_instr t_fact_typ) -∗
+    (N.of_nat f_myrec) ↦[wf] FC_func_native i (Tf [T_i32] []) [] (myrec_instr mut_tab) -∗
+    (N.of_nat f_mut_tab) ↦[wf] FC_func_host (Tf [T_i32; T_i32] []) (Mk_hostfuncidx mt) -∗
+    (N.of_nat mt) ↦[ha] HA_modify_table -∗
+    (N.of_nat tab) ↦[wt][N.of_nat (yy 0)] tabval -∗
+    (N.of_nat g_glob) ↦[wg] {| g_mut := MUT_mut; g_val := VAL_int32 n |} -∗
+    (N.of_nat idnstart) ↦[wf]FC_func_native i (Tf [] []) [] (main_instr fact glob) -∗
+                                                                                                                                                              
+    WP (([], [AI_invoke idnstart]) : host_expr) {{ Φ }}.
+    (* WP (([],to_e_list (main_instr fact glob)) : host_expr) {{ v, ∃ w, ⌜v = immHV []⌝ *)
+    (*                                                              ∗ fact_val n (immV [w]) *)
+    (*                                                              ∗ (N.of_nat g_glob) ↦[wg] {| g_mut := MUT_mut; g_val := w |} }}. *)
+  Proof.
+    iIntros (Hfact HF Hmyrec Hmut_tab Ht Htab Hglob Hoverflow Hpos).
+    iIntros "HΦ Hf Hfact HF Hmyrec Hmut_tab Hmt Htab Hg Hstart".
+    (* host bind *)
+    iApply wp_lift_wasm.
+    (* invoke main *)
+    take_drop_app_rewrite 0.
+    iApply (wp_invoke_native with "[$] [$]");eauto.
+    iNext. iIntros "[Hf Hstart]".
+    (* local bind *)
+    iApply (wp_frame_bind with "[$]");auto.
+    iIntros "Hf".
+    (* block *)
+    take_drop_app_rewrite 0.
+    iApply (wp_block with "[$]");eauto.
+    iNext. iIntros "Hf".
+    (* label bind *)
+    build_ctx (to_e_list (main_instr fact glob)).
+    iApply wp_label_bind. simpl.
+    (* get_global *)
+    bind_seq_base_imm [AI_basic (BI_get_global glob)] with "[Hg Hf]".
+    iApply (wp_get_global with "[] [$] [$]");eauto.
+    iIntros (w) "[-> [Hg Hf]] /=".
+    (* call fact *)
+    build_ctx [AI_basic (BI_call fact)].
+    iApply (wp_call_ctx with "[$]");eauto.
+    iNext. iIntros "Hf".
+    deconstruct_ctx.
+    (* invoke f_fact *)
+    bind_seq_base_callhost [AI_basic (BI_const (VAL_int32 n)); AI_invoke f_fact] with "[Hf Hfact Hmyrec Htab Hmut_tab]".
+    { (* f_fact *)
+      take_drop_app_rewrite 1.
+      iApply (wp_invoke_native with "[$] [$Hfact]");eauto.
+      iNext. iIntros "[Hf Hfact]".
+      iApply (wp_frame_bind with "Hf");auto.
+      iIntros "Hf".
+      take_drop_app_rewrite 0.
+      iApply (wp_block with "[$]");auto.
+      iNext. iIntros "Hf".
+      erewrite app_nil_l.
+      build_ctx (to_e_list (fact_instr (VAL_int32 F) myrec t_fact_typ)).
+      iApply wp_label_bind.
+      (* get_local 0 *)
+      bind_seq_base_imm [AI_basic (BI_get_local 0)] with "[Hf]".
+      iApply (wp_get_local with "[] [$]");eauto.
+      iIntros (w) "[-> Hf] /=".
+      (* call myrec *)
+      build_ctx [AI_basic (BI_call myrec)].
+      iApply (wp_call_ctx with "[$]");eauto.
+      iNext. iIntros "Hf".
+      deconstruct_ctx.
+      (* invoke f_myrec *)
+      bind_seq_base_callhost [AI_basic (BI_const (VAL_int32 F)); AI_invoke f_myrec] with "[Hf Hmyrec Hmut_tab]".
+      { (* myrec *)
+        take_drop_app_rewrite 1.
+        iApply (wp_invoke_native with "[$] [$]");eauto.
+        iNext. iIntros "[Hf Hmyrec] /=".
+        iApply (wp_frame_bind with "Hf");auto.
+        iIntros "Hf".
+        take_drop_app_rewrite 0.
+        iApply (wp_block with "[$]");auto.
+        iNext. iIntros "Hf".
+        build_ctx (to_e_list (myrec_instr mut_tab)).
+        iApply wp_label_bind.
+        (* myrec body *)
+        iApply (wp_wand with "[Hf Hmut_tab]").
+        iApply (myrec_spec with "[$] [$]");eauto.
+        iIntros (v) "[[-> Hmut_tab] Hf]".
+        deconstruct_ctx.
+        iApply iris_wp.wp_value;[apply iris.of_to_val;eauto|].
+        iExists _. iSplitR "Hf";[|iFrame]. iIntros "Hf".
+        iApply wp_frame_rewrite.
+        iApply iris_wp.wp_value;[apply iris.of_to_val;eauto|].
+        iSplitR;eauto. iCombine "Hmyrec Hmut_tab Hf" as "HH". instantiate (1:=λ _,_). iExact "HH". }
+      iIntros (w) "[-> [Hmyrec [Hmut_tab Hf]]]".
+      (* iApply wp_base_pull. *)
+      (* iApply wp_wasm_empty_ctx. *)
+      iApply iris_wp.wp_value;[apply iris.of_to_val;eauto|].
+      deconstruct_ctx.
+      iApply iris_wp.wp_value;[apply iris.of_to_val;eauto|simpl].
+      iExists _. iFrame. iIntros "Hf".
+      iApply wp_frame_rewrite.
+      iApply iris_wp.wp_value;[apply iris.of_to_val;eauto|simpl].
+      iSplit;eauto.
+      iCombine "Htab Hfact Hmyrec Hmut_tab Hf" as "HH".
+      instantiate (1:=λ _, _). iExact "HH".
+    }
+    iIntros (w) "[-> [Htab [Hfact [Hmyrec [Hmut_tab Hf]]]]]".
+    iApply iris_wp.wp_value;[apply iris.of_to_val;eauto|simpl].
+    deconstruct_ctx.
+    iApply iris_wp.wp_value;[apply iris.of_to_val;eauto|simpl].
+    iExists _. iFrame. iIntros "Hf".
+    iApply iris_wp.wp_value;[apply iris.of_to_val;eauto|simpl].
+
+    iApply wp_call_host_modify_table;[eauto|build_llfill|simpl;reflexivity|eauto|eauto|].
+    iFrame. iNext. iIntros "[Hf [Ha Htab]]".
+
+    iApply wp_lift_wasm.
+    iApply (wp_frame_bind with "[$]");auto.
+    iIntros "Hf".
+    match goal with | |- context [ AI_local ?i ?f ?es :: ?e ] => set (P:=AI_local i f es :: e); set (l:=es) end.
+    build_ctx P.
+    iApply wp_label_bind.
+    bind_seq_base_imm [AI_local 1 {| f_locs := [VAL_int32 n]; f_inst := i |} l] with "[Hf Htab HF]".
+    { iApply (wp_frame_bind with "[$]");auto.
+      iIntros "Hf". subst l.
+      match goal with | |- context [ AI_label ?i ?f ?es ] => set (l:=es) end.
+      build_ctx l; subst l.
+      iApply wp_label_bind.
+      match goal with | |- context [ AI_local ?i ?f ?es ] => set (l:=es) end.
+      bind_seq_base_imm [AI_local 0 {| f_locs := [VAL_int32 F]; f_inst := i |} l] with "[Hf]";[subst l|].
+      { iApply (wp_frame_bind with "[$]");auto.
+        iIntros "Hf".
+        iApply (wp_wand _ _ _ (λ v, ⌜v = immV _⌝ ∗ _)%I with "[Hf]"). iApply (wp_label_value with "Hf");eauto.
+        iIntros (v) "[-> Hf]". iExists _. iFrame.
+        iIntros "Hf /=".
+        iApply (wp_frame_value with "[$]");eauto. }
+      iIntros (v) "[-> Hf] /=".
+      (* BI_call_indirect *)
+      build_ctx [AI_basic (BI_const (xx 0));AI_basic (BI_call_indirect t_fact_typ)].
+      iApply (wp_call_indirect_success_ctx with "[Htab] HF Hf");eauto.
+      iNext. iIntros "[Htab [HF Hf]]".
+      deconstruct_ctx.
+      (* invoke f_F *)
+      take_drop_app_rewrite 1.
+      iApply (wp_invoke_native with "[$] [$]");eauto.
+      iNext. iIntros "[Hf HF]".
+      (* f_F *)
+      iApply (wp_frame_bind with "[$]");auto.
+      iIntros "Hf".
+      take_drop_app_rewrite 0. iApply (wp_block with "[$]");eauto.
+      iNext. iIntros "Hf".
+      build_ctx (to_e_list (F_instr t_fact_typ)).
+      iApply wp_label_bind.
+      iApply (wp_wand with "[-]").
+      iApply (F_spec with "[$] [$] [$]");eauto.
+      iIntros (v) "[[%Hspec [Htab HF]] Hf]".
+      rewrite Hspec.
+      (* return from block and frame *)
+      iApply (wp_val_return with "[$]");auto.
+      iIntros "Hf".
+      iApply iris_wp.wp_value;[unfold IntoVal;eapply iris.of_to_val;eauto|].
+      iExists _. iFrame. iIntros "Hf".
+      iApply (wp_wand _ _ _ (λ v, ⌜v = _⌝ ∗ _ )%I with "[Hf]").
+      iApply (wp_frame_value with "[$]");eauto.
+      iIntros (v') "[-> Hf]". rewrite Hspec.
+      iApply (wp_val_return with "[$]");auto.
+      iIntros "Hf /=".
+      iApply iris_wp.wp_value;[unfold IntoVal;eapply iris.of_to_val;rewrite Hspec;eauto|].
+      iExists _. iFrame. iIntros "Hf".
+      iApply (wp_wand _ _ _ (λ v, ⌜v = immV _⌝ ∗ _ )%I with "[Hf]").
+      iApply (wp_frame_value with "[$]");rewrite Hspec;auto.
+      iIntros (v') "[-> Hf]".
+      iSplit;[eauto|].
+      iCombine "Htab HF Hf" as "HH". instantiate (1:=λ _, _). iExact "HH".
+    }
+    iIntros (v) "[-> [Htab [HF Hf]]] /=".
+    iApply (wp_wand _ _ _ (λ v, ⌜v = immV _⌝ ∗ _)%I with "[Hg Hf]").
+    iApply (wp_set_global with "[] [$] [$]");eauto.
+    iIntros (v) "[-> [Hg Hf]]".
+    iApply (wp_val_return with "[$]");auto.
+    iIntros "Hf /=".    
+    iApply iris_wp.wp_value;[unfold IntoVal;eapply iris.of_to_val;eauto|].
+    iExists _. iFrame. iIntros "Hf".
+    iApply (wp_wand _ _ _ (λ v, ⌜v = immV _⌝ ∗ _ )%I with "[Hf]").
+    iApply (wp_frame_value with "[$]");eauto.
+    iIntros (v) "[-> Hf]".
+    iApply wp_value;eauto.
+    iApply "HΦ". eauto.
+  Qed.
+    
+End FactorialHostMain.
+
+Section FactorialHost.
+  Context `{!wasmG Σ, !hvisG Σ, !hmsG Σ, !hasG Σ}.
+
+  Definition factorial_module :=
+    {|
+      mod_types := [ Tf [T_i32] [T_i32] ; Tf [T_i32] [] ; Tf [T_i32; T_i32] [] ; Tf [] [] ] ;
+      mod_funcs :=
+      [ {|
+          modfunc_type := Mk_typeidx 1 ;
+          modfunc_locals := [] ;
+          modfunc_body := myrec_instr 0
+        |};
+        {|
+          modfunc_type := Mk_typeidx 0 ;
+          modfunc_locals := [] ;
+          modfunc_body := F_instr 0
+        |};
+        {|
+          modfunc_type := Mk_typeidx 0 ;
+          modfunc_locals := [] ;
+          modfunc_body := fact_instr (xx 2) 1 0
+        |};
+        {|
+          modfunc_type := Mk_typeidx 3 ;
+          modfunc_locals := [] ;
+          modfunc_body := main_instr 3 0
+        |}
+      ] ;
+      mod_tables := [ {| modtab_type := {| tt_limits := {| lim_min := 1 ; lim_max := None |} ; tt_elem_type := ELT_funcref |} |} ] ; 
+      mod_mems := [] ;
+      mod_globals := [ (* {| modglob_type := {| tg_mut := MUT_mut ; tg_t := T_i32 |} ; modglob_init := [BI_const (xx 0)] |} *) ] ;
+      mod_elem := [] ;
+      mod_data := [] ;
+      mod_start := Some (Build_module_start (Mk_funcidx 4)) ;
+      mod_imports :=
+        [ {|
+            imp_module := list_byte_of_string "Host" ;
+            imp_name := list_byte_of_string "modify_table" ;
+            imp_desc := ID_func 2
+          |};
+          {|
+            imp_module := list_byte_of_string "Host" ;
+            imp_name := list_byte_of_string "ret" ;
+            imp_desc := ID_global {| tg_mut := MUT_mut ; tg_t := T_i32 |}
+          |}
+        ];
+      mod_exports := []
+    |}.
+
+  Definition factorial_impts : seq.seq extern_t := [ET_func (Tf [T_i32; T_i32] []); ET_glob {| tg_mut := MUT_mut ; tg_t := T_i32 |}].
+
+  Ltac type_next_rewrite :=
+  match goal with
+  | |- context [ be_typing _ ?e _  ] =>
+      rewrite -(list.take_drop (length e - 1) e);simpl take; simpl drop
+  end.
+  Ltac type_next :=
+  match goal with
+  | |- context [ be_typing _ ?e _  ] =>
+      rewrite -(list.take_drop (length e - 1) e);simpl take; simpl drop;
+      eapply bet_composition;[|econstructor;eauto];simpl
+  end.
+  Ltac weaken :=
+  match goal with
+  | |- context [ be_typing _ ?e (Tf ?t1 ?t)  ] =>
+      try rewrite <- (app_nil_r t1);
+      rewrite -(list.take_drop (length t - 1) t);simpl take; simpl drop;
+      eapply bet_weakening;constructor;auto
+  end.
+  Ltac type_go := repeat (constructor || type_next || weaken || (type_next_rewrite; eapply bet_composition; [constructor|])).
+
+  Lemma factorial_module_typing :
+    module_typing factorial_module (factorial_impts) [].
+  Proof. unfold module_typing.
+    exists [Tf [T_i32] []; Tf [T_i32] [T_i32]; Tf [T_i32] [T_i32]; Tf [] []],[ (* {| tg_mut := MUT_mut ; tg_t := T_i32 |} *) ]. simpl.
+    repeat split;eauto.
+    { rewrite ! Forall2_cons. repeat split;auto; cbn;auto.
+      { type_go. }
+      { type_go.
+        type_next_rewrite.
+        eapply bet_composition. instantiate (1:=[T_i32]).
+        type_next_rewrite.
+        eapply bet_composition. instantiate (1:=[T_i32;T_i32]).
+        type_next_rewrite.
+        eapply bet_composition. instantiate (1:=[T_i32]).
+        type_next_rewrite.
+        eapply bet_composition. instantiate (1:=[T_i32;T_i32]).
+        all: type_go. }
+      { type_go.
+        type_next_rewrite.
+        eapply bet_composition. instantiate (1:=[T_i32]).
+        type_next_rewrite.
+        eapply bet_composition. instantiate (1:=[T_i32;T_i32]).
+        type_go. rewrite <- (app_nil_r [T_i32]).
+        rewrite -(list.take_drop (1) [T_i32;T_i32]);simpl take; simpl drop.
+        eapply bet_weakening.
+        type_go.
+        weaken. }
+      { type_go. }
+    }
+    { rewrite ! Forall2_cons. repeat split;auto; cbn;auto. }
+  Qed.
+
+  Definition factorial_module_instantiate :=
+    [ ID_instantiate [] 0 [0%N;1%N] ].
+
+  Notation "{{{ P }}} es {{{ v , Q }}}" :=
+    (□ ∀ Φ, P -∗ (∀ v, Q -∗ Φ v) -∗ WP (es : host_expr) @ NotStuck ; ⊤ {{ v, Φ v }})%I (at level 50).
+
+  Lemma instantiate_factorial hidx gidx mod_tab n :
+    (ssrnat.factorial (Wasm_int.nat_of_uint i32m n) < Wasm_int.Int32.modulus)%Z -> (* no overflow *)
+    (0 <= (Wasm_int.Int32.intval n))%Z -> (* the parameter must be positive *)
+    
+    ⊢ {{{ (N.of_nat hidx) ↦[wf] (FC_func_host (Tf [T_i32; T_i32] []) (Mk_hostfuncidx mod_tab)) ∗
+          (N.of_nat mod_tab) ↦[ha] HA_modify_table ∗
+          (N.of_nat gidx) ↦[wg] {| g_mut := MUT_mut; g_val := VAL_int32 n |} ∗
+          0%N ↪[mods] factorial_module ∗
+          (∃ name, 0%N ↪[vis] {| modexp_name := name; modexp_desc := MED_func (Mk_funcidx hidx) |}) ∗
+          (∃ name, 1%N ↪[vis] {| modexp_name := name; modexp_desc := MED_global (Mk_globalidx gidx) |}) ∗
+          ↪[frame] empty_frame
+      }}}
+        ((factorial_module_instantiate,[]) : host_expr) 
+      {{{ v, ⌜v = immHV []⌝ ∗ ∃ w, fact_val n (immV [w]) ∗ (N.of_nat gidx) ↦[wg] {| g_mut := MUT_mut; g_val := w |} }}} .
+  Proof.
+    iIntros (Hoverflow Hpos Φ). iModIntro. iIntros "(Hmod_tab & HA & Hglob & Hmod & Hvis1 & Hvis2 & Hf) HΦ".
+    iDestruct "Hvis1" as (name1) "Hvis1".
+    iDestruct "Hvis2" as (name2) "Hvis2".
+    iApply (instantiation_spec_operational_start_seq with "[$Hf] [$Hmod Hvis1 Hvis2 Hmod_tab Hglob] [HΦ HA]") => //.
+    { apply factorial_module_typing. }
+    { unfold module_restrictions. cbn. repeat split;exists [];auto. }
+    { cbn. instantiate (5:=[_;_]).
+      instantiate (1:={[N.of_nat gidx := {| g_mut := MUT_mut; g_val := VAL_int32 n |} ]}).
+      instantiate (1:=∅).
+      instantiate (1:=∅).
+      instantiate (1:= {[N.of_nat hidx := _ ]}).
+      iSplitL "Hvis1 Hvis2";[|iSplit;[|auto]].
+      simpl. iFrame. done.
+      rewrite /instantiation_resources_pre_wasm /=.
+      iSplitL;[|iPureIntro;split;apply Forall_nil;auto].
+      iSplitL "Hmod_tab";[|iSplitR;[|iSplitR]].
+      { rewrite /import_func_wasm_check /func_typecheck ! Forall2_cons /=.
+        iSplit. iApply big_sepM_singleton. iFrame. iPureIntro.
+        repeat split; auto. eexists _. rewrite lookup_singleton. eauto. set_solver. set_solver. }
+      { iSplit. by iApply big_sepM_empty. iPureIntro.
+        rewrite /tab_typecheck /tab_domcheck /factorial_impts ! Forall2_cons /=.
+        repeat split; auto. }
+      { iSplit. by iApply big_sepM_empty. iPureIntro.
+        rewrite /mem_typecheck /mem_domcheck /factorial_impts ! Forall2_cons /=.
+        repeat split; auto. }
+      { rewrite /import_glob_wasm_check /glob_typecheck ! Forall2_cons /=.
+        iSplit. iApply big_sepM_singleton. iFrame. iPureIntro.
+        repeat split; auto. eexists _. rewrite lookup_singleton. eauto. set_solver. set_solver. }
+    }
+
+    iIntros (idnstart) "Hf [Hmod [[Hvis1 [Hvis2 _]] Hi]]".
+    iDestruct "Hi" as (i) "[Hi _]".
+    unfold instantiation_resources_post_wasm.
+    iDestruct "Hi" as (g_inits tab_allocs mem_allocs glob_allocs wts' wms')
+                        "(Hres & %Hpre & %Htaballocs & %Hwts' & %Hcheck1
+                          & %Hmemalloc & %Hwms' & %Hcheck2 & %Hinit & %Hgloballocs & [Hfuncs [Htab [_ _]]])".
+    simplify_eq. destruct i. cbn in *.
+    destruct Hpre as [Htypes [Hprefuncs [_ [_ [Hpreglobs Hstart]]]]].
+    repeat (destruct inst_funcs;[done|]).
+    destruct inst_globs;[by inversion Hpreglobs|].
+    apply b2p in Hstart.
+    apply prefix_cons_inv_1 in Hprefuncs.
+    apply prefix_cons_inv_1 in Hpreglobs.
+    simplify_eq.
+    iDestruct "Hfuncs" as "[Hmyrec [HF [Hfact [Hmain _]]]] /=".
+
+    set (i:={| inst_types := [Tf [T_i32] [T_i32]; Tf [T_i32] []; Tf [T_i32; T_i32] []; Tf [] []];
+               inst_funcs := [:: f, f0, f1, f2, idnstart & inst_funcs];
+               inst_tab := inst_tab;
+               inst_memory := inst_memory;
+               inst_globs := g :: inst_globs
+            |}).
+    rewrite -/i.
+
+    rewrite drop_0. iDestruct (big_sepL2_length with "Htab") as %Htablen. destruct inst_tab;[done|].
+    iDestruct "Htab" as "[[[Ht _] _] _]".
+
+    iDestruct "Hres" as "[[Hmodtab _] [_ [_ [Hglob _]]]]".
+    rewrite /import_func_resources /import_glob_resources !big_sepM_singleton.
+
+    iApply (main_host_spec with "[$] [$] [$] [$] [$] [$] [$] [$] [$]");eauto;unfold i;simpl;auto.
+  Qed.
+    
+    
+End FactorialHost.
