theories/iris/rules/proofmode.v
@@ -1,0 +1,259 @@
+From mathcomp Require Import ssreflect eqtype seq ssrbool.
+From iris.program_logic Require Import language.
+From iris.proofmode Require Import base tactics classes.
+From iris.bi Require Export weakestpre.
+Require Export iris iris_locations iris_properties iris_atomicity stdpp_aux.
+Require Export iris_rules iris_example_helper.
+Require Export datatypes operations properties opsem.
+
+Set Implicit Arguments.
+Unset Strict Implicit.
+Unset Printing Implicit Defensive.
+
+Close Scope byte_scope.
+
+Lemma build_llfill_local n f llh es e l1 l2 :
+  llfill llh e = es ->
+  llfill (LL_local l1 n f llh l2) e = (v_to_e_list l1) ++ [AI_local n f es] ++ l2.
+Proof.
+  simpl. intros ->. auto.
+Qed.
+Lemma build_llfill_label n es' llh es e l1 l2 :
+  llfill llh e = es ->
+  llfill (LL_label l1 n es' llh l2) e = (v_to_e_list l1) ++ [AI_label n es' es] ++ l2.
+Proof.
+  simpl. intros ->. auto.
+Qed.
+Lemma build_llfill_base l1 l2 e :
+  llfill (LL_base l1 l2) e = (v_to_e_list l1) ++ e ++ l2.
+Proof. simpl. auto. Qed.
+
+Class DecomposeLocal (l: list administrative_instruction) l1 n f es l2 :=
+  { MkDecomposeLocal: l = (v_to_e_list l1) ++ [AI_local n f es] ++ l2 }.
+
+Hint Mode DecomposeLocal ! - - - - - : typeclass_instances.
+
+Instance DecomposeLocalConsHere : forall n f es l2, DecomposeLocal (AI_local n f es :: l2) [] n f es l2.
+Proof. intros. constructor. auto. Qed.
+
+Instance DecomposeLocalCons : forall n f es l2 l l' e, DecomposeLocal l2 l n f es l' -> DecomposeLocal ((AI_basic (BI_const e)) :: l2) (e :: l) n f es l'.
+Proof.
+  intros. constructor. inversion H. rewrite MkDecomposeLocal0.
+  simpl. auto.
+Qed.
+
+Lemma decompose_local_list l l1 l2 es n f :
+  DecomposeLocal l l1 n f es l2 ->
+  l = v_to_e_list l1 ++ [AI_local n f es] ++ l2.
+Proof.
+  intros D. destruct D. auto.
+Qed.
+
+Ltac build_llfill_local :=
+  match goal with
+  | |- context [ llfill _ _ = ?l ] =>
+      erewrite (decompose_local_list);[|once (typeclasses eauto)];
+      apply build_llfill_local
+  end.
+
+Class DecomposeLabel (l: list administrative_instruction) l1 n f es l2 :=
+  { MkDecomposeLabel: l = (v_to_e_list l1) ++ [AI_label n f es] ++ l2 }.
+
+Hint Mode DecomposeLabel ! - - - - - : typeclass_instances.
+
+Instance DecomposeLabelConsHere : forall n f es l2, DecomposeLabel (AI_label n f es :: l2) [] n f es l2.
+Proof. intros. constructor. auto. Qed.
+
+Instance DecomposeLabelCons : forall n f es l2 l l' e, DecomposeLabel l2 l n f es l' -> DecomposeLabel ((AI_basic (BI_const e)) :: l2) (e :: l) n f es l'.
+Proof.
+  intros. constructor. inversion H. rewrite MkDecomposeLabel0.
+  simpl. auto.
+Qed.
+
+Lemma decompose_label_list l l1 l2 es n f :
+  DecomposeLabel l l1 n f es l2 ->
+  l = v_to_e_list l1 ++ [AI_label n f es] ++ l2.
+Proof.
+  intros D. destruct D. auto.
+Qed.
+
+Ltac build_llfill_label :=
+  match goal with
+  | |- context [ llfill _ _ = ?l ] =>
+      erewrite (decompose_label_list);[|typeclasses eauto];
+      apply build_llfill_label
+  end.
+
+Class DecomposeBase l e l1 l2 :=
+  { MkDecomposeBase: l = (v_to_e_list l1) ++ e ++ l2 }.
+
+Hint Mode DecomposeBase ! ! - - : typeclass_instances.
+
+(* Instance DecomposeBaseAppHere : forall e l2, DecomposeBase (e ++ l2) e [] l2. *)
+(* Proof. intros. constructor. auto. Qed. *)
+
+Instance DecomposeBaseConsSingletonHere : forall e l2, DecomposeBase (e :: l2) [e] [] l2.
+Proof. intros. constructor. auto. Qed.
+
+Instance DecomposeBaseConsHere : forall l e es l2, DecomposeBase l es [] l2 -> DecomposeBase (e :: l) (e :: es) [] l2.
+Proof. intros. constructor. inversion H;subst. simpl. auto. Qed.
+
+Instance DecomposeBaseCons : forall l l1 e l2 e', DecomposeBase l e l1 l2 -> DecomposeBase ((AI_basic (BI_const e')) :: l) e (e' :: l1) l2.
+Proof. intros. inversion H. constructor. subst. simpl. auto. Qed.
+
+Lemma decompose_base_list l e l1 l2 :
+  DecomposeBase l e l1 l2 ->
+  l = v_to_e_list l1 ++ e ++ l2.
+Proof.
+  intros. inversion H. auto.
+Qed.
+
+Ltac build_llfill_base :=
+  match goal with
+  | |- context [ llfill _ _ = ?l ] =>
+      erewrite (@decompose_base_list l [AI_call_host _ _ _]);[|once (typeclasses eauto)];
+      apply build_llfill_base
+  end.
+
+Ltac build_llfill :=
+  repeat (build_llfill_local + build_llfill_label + build_llfill_base).
+
+Class BuildCtx i lh es LI :=
+  { MkBuildCtx: lfilled i lh es LI }.
+
+Hint Mode BuildCtx - - ! ! : typeclass_instances.
+
+Class DeconstructCtx i lh es LI :=
+  { MkDeconstruct: lfilled i lh es LI }.
+
+Hint Mode DeconstructCtx - - ! - : typeclass_instances.
+
+Instance DeconstructCtxBaseApp :
+  forall es l1 l2,
+    DeconstructCtx 0 (LH_base (v_to_e_list l1) l2) es (v_to_e_list l1 ++ es ++ l2).
+Proof.
+  intros.
+  constructor. apply lfilled_Ind_Equivalent. constructor.
+  apply v_to_e_is_const_list.
+Qed.
+
+Instance BuildCtxBase :
+  forall LI es l1 l2,
+    DecomposeBase LI es l1 l2 ->
+    BuildCtx 0 (LH_base (v_to_e_list l1) l2) es LI.
+Proof.
+  intros.
+  inversion H as [Heq]. subst.
+  constructor. apply lfilled_Ind_Equivalent. constructor.
+  apply v_to_e_is_const_list.
+Qed.
+
+Instance DeconstructCtxLabelApp :
+  forall l1 n es es' e l2 i lh,
+    DeconstructCtx i lh e es ->
+    DeconstructCtx (S i) (LH_rec (v_to_e_list l1) n es' lh l2) e ((v_to_e_list l1) ++ [AI_label n es' es] ++ l2).
+Proof.
+  intros until lh. intros B.
+  inversion B as [fill%lfilled_Ind_Equivalent].
+  constructor. apply lfilled_Ind_Equivalent.
+  constructor;auto.
+  apply v_to_e_is_const_list.
+Qed.
+
+Instance BuildCtxLabel :
+  forall LI l1 n es es' e l2 i lh,
+    DecomposeLabel LI l1 n es' es l2 ->
+    BuildCtx i lh e es ->
+    BuildCtx (S i) (LH_rec (v_to_e_list l1) n es' lh l2) e LI.
+Proof.
+  intros until lh. intros D B.
+  inversion D as [Heq].
+  inversion B as [fill%lfilled_Ind_Equivalent].
+  constructor. apply lfilled_Ind_Equivalent.
+  rewrite Heq. constructor;auto.
+  apply v_to_e_is_const_list.
+Qed.
+
+Lemma wp_build_ctx `{!wasmG Σ} es i lh LI s E P :
+  BuildCtx i lh es LI ->
+  WP es @ s; E CTX i; lh {{ P }} -∗ WP LI @ s; E {{ P }}.                                  
+Proof.
+  iIntros (B) "W".
+  inversion B as [fill].
+  iDestruct ("W" $! _ fill) as "W".
+  iFrame.
+Qed.
+
+Lemma wp_deconstruct_ctx `{!wasmG Σ} es i lh LI s E P :
+  DeconstructCtx i lh es LI ->
+  WP LI @ s; E {{ P }} -∗ WP es @ s; E CTX i; lh {{ P }}.
+Proof.
+  iIntros (B) "W".
+  inversion B as [fill].
+  iIntros (LI' fill').
+  eapply lfilled_inj in fill;eauto. subst.
+  iFrame.
+Qed.
+
+Ltac build_ctx e :=
+  match goal with
+  | |- context [ (WP ?es @ ?s; ?E {{ ?P }})%I ] =>
+      iApply (@wp_build_ctx _ _ e)
+  end.
+
+Ltac deconstruct_ctx :=
+  match goal with
+  | |- context [ (WP ?es @ ?s; ?E CTX ?i; ?lh {{ ?P }})%I ] =>
+      iApply (@wp_deconstruct_ctx _ _ es);
+      try (constructor;cbn;rewrite eqseqE;eauto);
+      iSimpl
+  end.
+
+Lemma bind_seq_base_imm `{!wasmG Σ} es P LI l1 l2 s E Q w :
+  DecomposeBase LI es l1 l2 ->
+  WP es @ E {{ λ v, ⌜v = immV w⌝ ∗ P v }}
+  -∗ (∀ v, ⌜v = immV w⌝ ∗ P v
+                -∗ WP (v_to_e_list l1) ++ (iris.of_val v) ++ l2 @ s; E {{ Q }})
+  -∗ WP LI @ s; E {{ Q }}.
+Proof.
+  intros. iIntros "H1 H2".
+  build_ctx es.
+  rewrite <- (app_nil_r es).
+  iApply (wp_seq_ctx s E Q (λ v, ⌜v = immV _⌝ ∗ _)%I es).
+  iSplitR;[by iIntros "[%Hcontr _]"|].
+  rewrite app_nil_r. iFrame.
+  iIntros (v') "H".
+  rewrite app_nil_r.
+  iApply wp_base_pull. iApply wp_wasm_empty_ctx.
+  iApply "H2". iFrame.
+Qed.
+
+Lemma bind_seq_base_callhost `{!wasmG Σ} es P LI l1 l2 s E Q a1 a2 a3 a4 :
+  DecomposeBase LI es l1 l2 ->
+  WP es @ E {{ λ v, ⌜v = callHostV a1 a2 a3 a4⌝ ∗ P v }}
+  -∗ (∀ v, ⌜v = callHostV a1 a2 a3 a4⌝ ∗ P v -∗ WP (v_to_e_list l1) ++ (iris.of_val v) ++ l2 @ s; E {{ Q }})
+  -∗ WP LI @ s; E {{ Q }}.
+Proof.
+  intros. iIntros "H1 H2".
+  build_ctx es.
+  rewrite <- (app_nil_r es).
+  iApply (wp_seq_ctx s E Q (λ v, ⌜v = callHostV a1 a2 a3 a4⌝ ∗ _)%I es).
+  iSplitR;[by iIntros "[%Hcontr _]"|].
+  rewrite app_nil_r. iFrame.
+  iIntros (v') "H".
+  rewrite app_nil_r.
+  iApply wp_base_pull. iApply wp_wasm_empty_ctx.
+  iApply "H2". iFrame.
+Qed.
+
+Ltac bind_seq_base_imm e h :=
+  iApply (@bind_seq_base_imm _ _ e with h).
+
+Tactic Notation "bind_seq_base_imm" constr(e) "with" constr(h) :=
+  bind_seq_base_imm e h.
+
+Ltac bind_seq_base_callhost e h :=
+  iApply (@bind_seq_base_callhost _ _ e with h).
+
+Tactic Notation "bind_seq_base_callhost" constr(e) "with" constr(h) :=
+  bind_seq_base_callhost e h.
